%% Font size %%
\documentclass[11pt]{article}

%% Load the custom package
\usepackage{Mathdoc}

%% Numéro de séquence %% Titre de la séquence %%
\renewcommand{\centerhead}{Caluls sur les puissances avec des relatifs}

%% Spacing commands %%
\renewcommand{\baselinestretch}{1} \setlength{\parindent}{0pt}

\begin{document}


\begin{exercice}[1]
\begin{multicols}{2}
\begin{enumerate}[itemsep=1em]
\item  $A=(-3)^{5}\times (-3)^{2}=$
\item  $B=(-4)^{4}\times (-4)^{3}=$
\item  $C=(-5)^{3}\times (-5)^{2}=$
\item  $D=(-3)^{5}\times (-3)^{3}=$
\item  $E=(-4)^{3}\times (-4)^{2}=$
\item  $F=(-4)^{5}\times (-4)^{3}=$
\item  $G=(-3)^{3}\times (-3)^{2}=$
\item  $H=(-6)^{4}\times (-6)^{2}=$
\item  $I=(-2)^{4}\times (-2)^{3}=$
\item  $J=(-5)^{5}\times (-5)^{2}=$
\end{enumerate}
\end{multicols}
\end{exercice}


\begin{exercice}[1]
\begin{multicols}{2}
\begin{enumerate}[itemsep=2em]
\item  $A=\dfrac{(-8)^{3}}{(-8)^{2}}=$
\item  $B=\dfrac{(-2)^{5}}{(-2)^{4}}=$
\item  $C=\dfrac{(-3)^{4}}{(-3)^{3}}=$
\item  $D=\dfrac{(-8)^{5}}{(-8)^{4}}=$
\item  $E=\dfrac{(-7)^{4}}{(-7)^{2}}=$
\item  $F=\dfrac{(-6)^{5}}{(-6)^{2}}=$
\item  $G=\dfrac{(-5)^{4}}{(-5)^{2}}=$
\item  $H=\dfrac{(-4)^{3}}{(-4)^{2}}=$
\item  $I=\dfrac{(-3)^{3}}{(-3)^{2}}=$
\item  $J=\dfrac{(-6)^{4}}{(-6)^{2}}=$
\end{enumerate}
\end{multicols}
\end{exercice}


\begin{exercice}[1]
\begin{multicols}{2}
\begin{enumerate}[itemsep=1.5em]
\item  $A=(7^{4})^{2}=$
\item  $B=(7^{2})^{2}=$
\item  $C=((-2)^{2})^{2}=$
\item  $D=((-2)^{3})^{3}=$
\item  $E=(8^{2})^{3}=$
\item  $F=(4^{4})^{2}=$
\item  $G=((-2)^{4})^{3}=$
\item  $H=((-3)^{4})^{4}=$
\item  $I=((-8)^{4})^{2}=$
\item  $J=(8^{3})^{3}=$
\end{enumerate}
\end{multicols}
\end{exercice}


\begin{exercice}[1]
\begin{multicols}{2}
\begin{enumerate}[itemsep=1.5em]
\item  $A=8^{3}\times 5^{3}=$
\item  $B=(-3)^{5}\times (-7)^{5}=$
\item  $C=7^{3}\times 5^{3}=$
\item  $D=(-7)^{5}\times 5^{5}=$
\item  $E=8^{3}\times 3^{3}=$
\item  $F=5^{3}\times 8^{3}=$
\item  $G=(-5)^{2}\times 3^{2}=$
\item  $H=2^{4}\times 5^{4}=$
\item  $I=(-2)^{4}\times 8^{4}=$
\item  $J=(-5)^{2}\times (-3)^{2}=$
\end{enumerate}
\end{multicols}
\end{exercice}


\begin{exercice}[1]
\begin{multicols}{2}
\begin{enumerate}[itemsep=2em]
\item  $A=\dfrac{15^{5}}{(-5)^{5}}=$
\item  $B=\dfrac{(-20)^{2}}{(-5)^{2}}=$
\item  $C=\dfrac{(-6)^{4}}{(-2)^{4}}=$
\item  $D=\dfrac{(-12)^{2}}{(-3)^{2}}=$
\item  $E=\dfrac{(-8)^{2}}{(-2)^{2}}=$
\item  $F=\dfrac{(-6)^{4}}{2^{4}}=$
\item  $G=\dfrac{6^{4}}{2^{4}}=$
\item  $H=\dfrac{(-9)^{4}}{3^{4}}=$
\item  $I=\dfrac{(-4)^{3}}{(-2)^{3}}=$
\item  $J=\dfrac{8^{2}}{2^{2}}=$
\end{enumerate}
\end{multicols}
\end{exercice}

\end{document}
